examples/layeredeffects/HoareSTPolyBind.fst
@@ -136,7 +136,7 @@ let get ()
   (fun h0 h h1 -> h0 == h1 /\ h == h1)
 = HoareST?.reflect get
 
-assume val wp_monotonic_pure (_:unit)
+assume val elim_pure_wp_monotonicity_forall (_:unit)
   : Lemma
     (forall (a:Type) (wp:pure_wp a).
        (forall (p q:pure_post a).
@@ -154,7 +154,7 @@ let bind_pure_hoarest (a:Type) (b:Type) (wp:pure_wp a) (req:a -> pre_t) (ens:a -
 : repr b
   (fun h -> wp (fun x -> req x h))
   (fun h0 r h1 -> exists x. (~ (wp (fun r -> r =!= x))) /\ ens x h0 r h1)
-= wp_monotonic_pure ();
+= elim_pure_wp_monotonicity_forall ();
   fun _ ->
   let x = f () in
   g x ()
@@ -168,7 +168,7 @@ let bind_hoarest_pure (a:Type) (b:Type) (req:pre_t) (ens:post_t a) (wp:a -> pure
 : repr b
   (fun h -> req h /\ (forall x h1. ens h x h1 ==> (wp x) (fun _ -> True)))
   (fun h0 r h1 -> exists x. ens h0 x h1 /\ (~ ((wp x) (fun y -> y =!= r))))
-= wp_monotonic_pure ();
+= elim_pure_wp_monotonicity_forall ();
   fun _ ->
   let x = f () in
   (g x) ()
@@ -187,7 +187,7 @@ let subcomp_pure_hoarest (a:Type) (wp:pure_wp a) (req:pre_t) (ens:post_t a)
     (forall h. req h ==>  wp (fun _ -> True)) /\
     (forall h0 r h1. (~ (wp (fun x -> x =!= r \/ h0 =!= h1))) ==>  ens h0 r h1))
   (ensures fun _ -> True)
-= wp_monotonic_pure ();
+= elim_pure_wp_monotonicity_forall ();
   fun _ -> f ()
 
 polymonadic_subcomp PURE <: HoareST = subcomp_pure_hoarest
