examples/layeredeffects/LowParseWriters.fsti
@@ -358,7 +358,7 @@ let lift_pure_read (a:Type) (wp:pure_wp a)
     (fun _ -> False) // (lift_pure_read_post_err a wp))
     l
   )
-= wp_monotonic_pure ();
+= elim_pure_wp_monotonicity_forall ();
   ReadRepr _ (lift_pure_read_impl a wp f_pure l)
 
 sub_effect PURE ~> ERead = lift_pure_read
